\documentclass[a4paper, 12pt]{article}
\usepackage[T1]{fontenc}
\usepackage[utf8]{inputenc}
\usepackage{geometry}
\usepackage{fancyhdr}
\usepackage{amssymb}

\pagestyle{fancy}
\fancyhf{}
\rhead{Makerere Univeristy | Kampala }
\lhead{\bfseries Michael Goboola  09/29/2000  Male }
\rfoot{}


\begin{document}

\begin{center}
    \fontsize{24pt}{10pt}\selectfont
    \textsc{\textbf{Attempted}}
\end{center}

\section{Question 1}
$a$  $\in$  $\mathbb{R}$, $b$  $\in$  $\mathbb{R}$ then by  the mapping $g$ , $g(a)$  $\in$ $\mathbb{R}$ and
g(b) $\in$ $\mathbb{R}$. Suppose a,b $\in$ $\mathbb{N}$ and $\mathbb{N}$ $\subset$ $\mathbb{R}$, 
then by the principle of recursive definition there exists a function $\phi$ such that
$\phi(a + b)$ = $\phi(a)$ + $\phi(b)$ and $\phi(ab)$ = $\phi(a)\phi(b)$.
If a = b , then $g(a)^2$ $\equiv$ $g(a)g(a$) $\equiv$ $g(a^2)$  and $g(a^2 + a + g(a))$ $\equiv$ $g(a^2)$ + g(a) + g(g(a)).
Then proceeding with contradiction taking from the problem we have:
\begin{center}
    $g(a^2 + b + g(b)) = 2b + g(a)^2$
    taking b = a, $\forall$ a,b $\in$ $\mathbb{N}$ $\subset$ $\mathbb{R}$
    by the principle of recursive definition
    $g(a)g(a) + g(a) + g(g(a)) = 2a + g(a)g(a)$
    $g(a) + g(g(a)) = 2a$
\end{center}
but since a $\in$ $\mathbb{N}$ and $\mathbb{N}$ $\subset$ $\mathbb{R}$ $\implies $ a $\in$ $\mathbb{R}$, 
but g(a) $\in$ $\mathbb{R}$ and the function compositon of $g(g(a))$ $\in$ $\mathbb{R}$ $\implies $ $g(a) + g(g(a))\neq$ $2a$
since the scaling a by $2$ where $2$ , a $\in$ $\mathbb{N}$ does not imply equality despite $\mathbb{N}$ $\subset$ $\mathbb{R}$ 
this contradiction it makes the function $g:\mathbb{R}\longrightarrow \mathbb{R}$ undefined in the ordered field $\mathbb{R}$ completes the proof. $\blacksquare$ 

\newpage

\section{Question 2}

\newpage

\section{Question 3}

\end{document}